chore: separate pointer invariants from the item invariants
Since the relevant creation functions are defined, there is no need to
have the invariant at the side and its fine to have it as a separate
theorem that the invariants get maintained.

Earley/Parser.lean
@@ -6,8 +6,10 @@ Authors: Daniel Soukup
 module
 public import Earley.Model
 public import Earley.Recognizer
+public import Earley.Proofs.Recognizer
 public import Earley.Filter
 public import Earley.CachedRecognizerPointers
+public import Earley.Proofs.CachedRecognizerPointers
 
 /-!
 This module represents a functional implementation of the Earley algorithm on the production of
@@ -21,6 +23,328 @@ https://doi.org/10.4230/LIPIcs.ITP.2024.31
 
 namespace Earley
 namespace Parser
+
+section Wellformed
+
+open Earley.Model
+open Earley.Model.EarleyItem
+open Earley.Recognizer
+open Earley.Proofs.Recognizer
+open Earley.Utils
+
+variable {T N : Type} [BEq T] [BEq N] [LawfulBEq (EarleyItem T N)]
+
+/--
+A pointer is well-formed with respect to an EarleyBins, if the pointer points to a stored bin item.
+`k` is the index of the bin, at which the pointer is stored at.
+
+Since reduction pointers can point towards any earlier bin than k, this is a very global property
+and difficult to reason about locally. This makes it too inconvenient to merge it with
+the soundness property about pointers.
+-/
+@[grind]
+public def Pointer.WF {w : Array T} (bins : EarleyBins T N (w.size + 1)) (pointer : Pointer)
+    (k : Nat) : Prop :=
+  match pointer with
+  | .null => True
+  | .predecessor i => k ≠ 0 ∧ k - 1 ≤ w.size ∧ ((h : k - 1 ≤ w.size) → i < bins[k-1].length)
+  | .reduction p ps => k ≤ w.size ∧ p.endIdxA ≤ w.size
+    ∧ ((h : p.endIdxA ≤ w.size) → p.i < bins[p.endIdxA].length)
+    ∧ ((h : k ≤ w.size) → p.j < bins[k].length)
+
+@[grind]
+public def BinPointers.WF {L : Type} {w : Array T} (bins : EarleyBins T N (w.size + 1))
+    (bin : L) [Membership (BinItem T N) L] (k : Nat) : Prop :=
+  ∀ x ∈ bin, Pointer.WF bins x.pointer k
+
+/--
+A pointer is called sound, if the reduction pointer points towards an earlier item.
+Interestingly enough, we only reason about the first pointer
+since it is the only one used for buildTree anyway.
+There are problematic details when merging reduction pointers since the item could in theory
+skip ahead of the item that triggered the .complete operation.
+-/
+@[grind]
+public def Pointer.isSound (pointer : Pointer) (k j : Nat) : Prop :=
+  match pointer with
+  | .null | .predecessor _ => True
+  | .reduction p _ => (p.endIdxA < k ∨ (p.endIdxA = k ∧ p.i < j)) ∧ p.j < j
+
+/--
+EarleyBins is well-formed w.r.t to their pointers, if all of its bins got well-formed pointers.
+-/
+@[grind]
+public def EarleyBins.PointerWF {w : Array T} (bins : EarleyBins T N (w.size + 1)) : Prop :=
+  ∀ k, (hk : k < bins.size) → BinPointers.WF bins bins[k] k
+   ∧ ∀ j, (hj : j < bins[k].length) → Pointer.isSound bins[k][j].pointer k j
+
+@[grind →]
+lemma updateBinAux_of_nullPre (xs : BinItems T N) (y : BinItem T N) {i : Nat}
+    (hmem : y.item ∈ items xs) (hy : y.pointer = .null ∨ y.pointer = .predecessor i) :
+    updateBinAux y xs = xs := by
+  induction xs generalizing y with
+  | nil => grind
+  | cons head tail ih => grind
+
+lemma eqLength_of_updateBinAux_of_mem (xs : BinItems T N) (y : BinItem T N)
+    (hNoDup : (items xs).Nodup) (hmem : y.item ∈ items xs) :
+    (updateBinAux y xs).length = xs.length := by
+  induction xs generalizing y with
+  | nil => grind
+  | cons x xs ih => grind
+
+lemma updateBinAux_of_Red_of_neqItemAux (xs : BinItems T N) (y : BinItem T N) (i : Nat)
+    (hi : i < xs.length) (hneq : y.item ≠ xs[i].item) (hlen : i < (updateBinAux y xs).length) :
+    (updateBinAux y xs)[i] = xs[i] := by
+  induction xs generalizing i with
+  | nil => grind
+  | cons x xs ih => grind
+
+lemma updateBinAux_of_Red_of_neqItem (xs : BinItems T N) (y : BinItem T N) (i j : Nat)
+    (hNoDup : (items xs).Nodup) (hi : i < xs.length) (heq : y.item = xs[i].item) (hneq : i ≠ j)
+    (hj : j < xs.length) (hlen : j < (updateBinAux y xs).length) :
+    (updateBinAux y xs)[j] = xs[j] := by
+  induction xs generalizing i with
+  | nil => grind
+  | cons x xs ih =>
+    have : y.item ≠ (x :: xs)[j].item := by
+      grind [List.nodup_iff_getElem?_ne_getElem?]
+    grind [updateBinAux_of_Red_of_neqItemAux]
+
+lemma updateBinAux_of_updRed (xs xs' : BinItems T N) (y : BinItem T N) (i : Nat)
+    (hNoDup : (items xs).Nodup) {xp yp : ReductionPointer} {xP yP : List ReductionPointer}
+    (hi : i < xs.length) (hx : xs[i].pointer = Pointer.reduction xp xP) (heq : y.item = xs[i].item)
+    (hy : y.pointer = .reduction yp yP) (hxs' : xs' = updateBinAux y xs) :
+    xs'.length = xs.length ∧ ((hlen : xs'.length = xs.length) →
+    xs'[i].pointer = .reduction xp (yp::yP.append xP) ∧
+    (∀ j, (hj : j < xs'.length ∧ i ≠ j) → xs'[j] = xs[j]'(by lia))) := by
+  induction xs generalizing i y xs' with
+  | nil => grind
+  | cons x xs ih =>
+    refine ⟨by grind [eqLength_of_updateBinAux_of_mem], ?_⟩
+    intro hlen
+    simp only [hxs', ne_eq, forall_and_index]
+    constructor
+    · grind
+    · intro j hk hneq
+      have := updateBinAux_of_Red_of_neqItem (x::xs) y i j
+      grind
+
+lemma updateBinAux_of_Red_of_eqItem (xs : BinItems T N) (y : BinItem T N) (i j : Nat)
+    (hNoDup : (items xs).Nodup) (hi : i < xs.length)
+    (hx : xs[i].pointer = .null ∨ xs[i].pointer = .predecessor j) (heq : y.item = xs[i].item) :
+    updateBinAux y xs = xs := by
+  induction xs generalizing i with
+  | nil => grind
+  | cons x xs ih => grind
+
+omit [BEq T] [BEq N] [LawfulBEq (EarleyItem T N)] in
+lemma wfBinPointers_of_updatedBins (w : Array T) {k : Nat}
+    (bins bins' : EarleyBins T N (w.size + 1)) (hk : k < w.size + 1)
+    (hbins' : ∀ i, (hi : i ≤ w.size) → bins[i].length ≤ bins'[i].length)
+    (h : BinPointers.WF bins bins'[k] k) : BinPointers.WF bins' bins'[k] k := by
+  simp only [BinPointers.WF]
+  simp only [BinPointers.WF] at h
+  intro x hmem
+  specialize h x hmem
+  simp only [Pointer.WF, ne_eq, tsub_le_iff_right]
+  simp only [Pointer.WF, ne_eq, tsub_le_iff_right] at h
+  split <;> grind
+
+omit [LawfulBEq (EarleyItem T N)] in
+lemma wfBinPointers_of_updateBinAux {w : Array T} {k : Nat} (bins : EarleyBins T N (w.size + 1))
+    (xs : BinItems T N) (hwfbin : BinPointers.WF bins xs k) (y : BinItem T N)
+    (hwfy : Pointer.WF bins y.pointer k) : BinPointers.WF bins (updateBinAux y xs) k := by
+  induction xs with
+  | nil => grind
+  | cons x xs ih => grind
+
+omit [LawfulBEq (EarleyItem T N)] in
+lemma wfBinPointers_of_updateBin (w : Array T) {k : Nat} (bins : EarleyBins T N (w.size + 1))
+    (xs : BinItems T N) (hwfbin : BinPointers.WF bins xs k)
+    (ys : BinItems T N) (hwfy : ∀ y ∈ ys, Pointer.WF bins y.pointer k) :
+    BinPointers.WF bins (updateBin xs ys) k := by
+  induction ys generalizing xs with
+  | nil => grind
+  | cons y ys ih =>
+    have hwfAux := wfBinPointers_of_updateBinAux bins xs hwfbin y (by grind)
+    grind
+
+lemma soundPointers_of_updateBinAux (wlen : Nat) {k : Nat} (bins : EarleyBins T N (wlen + 1))
+    (hbins : ∀ k, (hk : k ≤ wlen) → (items bins[k]).Nodup ∧ ∀ j, (hj : j < bins[k].length)
+      → Pointer.isSound bins[k][j].pointer k j)
+    (y : BinItem T N) (hk : k < wlen + 1) (hwf : Pointer.isSound y.pointer k bins[k].length) :
+    ∀ j, (hj : j < (updateBinAux y bins[k]).length) →
+    Pointer.isSound (updateBinAux y bins[k])[j].pointer k j := by
+  have : y.item ∉ items bins[k] ∨
+        (y.item ∈ items bins[k] ∧ ∃ i, y.pointer = .null ∨ y.pointer = .predecessor i) ∨
+        (y.item ∈ items bins[k] ∧ ¬ ∃ i, y.pointer = .null ∨ y.pointer = .predecessor i) := by
+    simp only [not_exists, not_or]
+    grind
+  rcases this with hnmem | ⟨hmem, hex⟩ | ⟨hmem, hnex⟩
+  · grind
+  · rcases hex with ⟨i,hi⟩
+    grind
+  · simp only [not_exists, not_or] at hnex
+    match hy : y.pointer with
+    | .null | .predecessor i => grind [hnex 0]
+    | .reduction yp yP =>
+      have := List.getElem_of_mem hmem
+      rcases this with ⟨j', hjI', heq⟩
+      have hj' : j' < bins[k].length := by grind
+      match hb : bins[k][j'].pointer with
+      | .null =>
+        have := (hbins k (by grind)).left
+        have heq' : y.item = bins[k][j'].item := by
+          simp only [items, List.getElem_map] at heq
+          simp [heq]
+        have := updateBinAux_of_Red_of_eqItem bins[k] y j' 0 this (by grind) (by simp [hb]) heq'
+        grind
+      | .predecessor i =>
+        have := (hbins k (by grind)).left
+        have heq' : y.item = bins[k][j'].item := by
+          simp only [items, List.getElem_map] at heq
+          simp [heq]
+        have := updateBinAux_of_Red_of_eqItem bins[k] y j' i this (by grind) (by simp [hb]) heq'
+        grind
+      | .reduction bp bP =>
+        have hnDup := (hbins k (by grind)).left
+        have : y.item = bins[k][j'].item := by grind
+        have hupdRed := updateBinAux_of_updRed bins[k] (updateBinAux y bins[k]) y j' hnDup hj'
+            hb this hy (by simp)
+        grind
+
+-- I cannot really simplify the goal and make the proof easier for me
+-- since any item of ys can get merged into the bins and thus the `< j` would get problematic.
+lemma soundPointers_of_updateBin (wlen : Nat) (k : Nat) (bins : EarleyBins T N (wlen + 1))
+    (hbins : ∀ k, (hk : k ≤ wlen) → (items bins[k]).Nodup ∧ ∀ j, (hj : j < bins[k].length)
+      → Pointer.isSound bins[k][j].pointer k j)
+    (ys : BinItems T N) (hk : k < wlen + 1)
+    (hwf : ∀ y ∈ ys, Pointer.isSound y.pointer k bins[k].length) :
+    ∀ j, (hj : j < (updateBin bins[k] ys).length) →
+    Pointer.isSound (updateBin bins[k] ys)[j].pointer k j := by
+  induction ys generalizing bins with
+  | nil => grind
+  | cons y ys ih =>
+    intro j hj
+    let bins' := Vector.set bins k (updateBinAux y bins[k]) hk
+    have hSaux := soundPointers_of_updateBinAux wlen bins hbins y hk (by grind)
+    have : ∀ y ∈ ys, Pointer.isSound y.pointer k bins'[k].length := by
+      clear ih
+      simp only [Pointer.isSound]
+      grind [length_le_lengthUpdateBinAux]
+    have hbins' : (∀ (k : ℕ) (hk : k ≤ wlen), (items bins'[k]).Nodup ∧
+        ∀ (j : ℕ) (hj : j < bins'[k].length), Pointer.isSound bins'[k][j].pointer k j) := by
+      clear this
+      intro k2 hk2
+      constructor
+      · grind [noDup_of_updateBinAux bins[k] y]
+      · grind
+    specialize ih bins' hbins' (by grind)
+    grind
+
+theorem pointerWF_of_updateBin (G : ContextFreeGrammarList T N) (w : Array T) {k : Nat}
+    (bins : EarleyBins T N (w.size + 1)) (hbins : EarleyBins.WF G bins)
+    (hwf : EarleyBins.PointerWF bins)
+    (ys : BinItems T N) (hk : k < w.size + 1)
+    (hwfPy : BinPointers.WF bins ys k)
+    (hwfSy : ∀ y ∈ ys, Pointer.isSound y.pointer k bins[k].length) :
+    EarleyBins.PointerWF (updateBins bins k ys)  := by
+  induction ys generalizing bins k with
+  | nil =>
+    have : Vector.modify bins k (fun x => x) = bins := by grind
+    grind
+  | cons y ys ih =>
+    simp [updateBins, EarleyBins.PointerWF]
+    refine ⟨by grind [soundPointers_of_updateBinAux, wfBinPointers_of_updateBinAux], by grind [soundPointers_of_updateBinAux, wfBinPointers_of_updateBinAux]⟩
+
+    --· have ⟨h0,h1,h2,h3⟩ := hwf k (by lia)
+    --  simp only [heq]
+    --  have hwfb : BinPointers.WF bins (updateBins bins k ys)[k] k := by
+    --    have := wfBinPointers_of_updateBin w bins bins[k] h2 ys (by grind)
+    --    grind
+    --  have : ∀ (i : ℕ) (hi : i ≤ w.size), bins[i].length
+    --      ≤ (updateBins bins k ys)[i].length := by grind [lengthNth_le_lengthUpdateBinNth]
+    --  have := wfBinPointers_of_updatedBins w bins (updateBins bins k ys) hk this hwfb
+    --  grind
+    --· intro j hj
+    --  have := soundPointers_of_updateBin w.size k bins (by grind) ys
+    --  grind
+  sorry
+
+omit [BEq N] [LawfulBEq (EarleyItem T N)] in
+lemma wfPointers_of_scanList {w : Array T} (j k : Nat) {a : T} {bins : EarleyBins T N (w.size + 1)}
+    (x : EarleyItem T N) (hk : k < w.size) (hj : ¬ (j ≥ bins[k].length)) :
+    BinPointers.WF bins (scanList w x a k hk j) (k+1) := by
+  grind [scanList]
+
+omit [BEq N] [LawfulBEq (EarleyItem T N)] in
+lemma soundPointers_of_scanList {w : Array T} (j k : Nat) {a : T}
+    {bins : EarleyBins T N (w.size + 1)} (x : EarleyItem T N) (hk : k < w.size) :
+    ∀ y ∈ scanList w x a k hk j, Pointer.isSound y.pointer (k+1) bins[k+1].length := by
+  grind [scanList]
+
+omit [BEq T] [LawfulBEq (EarleyItem T N)] in
+lemma wfPointers_of_predictList (G : ContextFreeGrammarList T N) (w : Array T) (k : Nat)
+    (A : N) {bins : EarleyBins T N (w.size + 1)} :
+    BinPointers.WF bins (predictList G A k) k := by
+  grind [predictList]
+
+omit [BEq T] [LawfulBEq (EarleyItem T N)] in
+lemma soundPointers_of_predictList (G : ContextFreeGrammarList T N) (wlen k : Nat) (A : N)
+    (bins : EarleyBins T N (wlen + 1)) (hk : k < wlen + 1) :
+    ∀ x ∈ predictList G A k, Pointer.isSound x.pointer k bins[k].length := by
+  grind [predictList]
+
+omit [LawfulBEq (EarleyItem T N)] in
+lemma wfPointers_of_completeList {G : ContextFreeGrammarList T N} (w : Array T) (j k : Nat)
+    {bins : EarleyBins T N (w.size + 1)} (hbins : EarleyBins.WF G bins) (y : EarleyItem T N)
+    (hk : k < bins.size) (hmemy : y ∈ (items bins[k])) (hj : j < bins[k].length) :
+    BinPointers.WF bins (completeList y bins (by grind) j) k := by
+  simp only [BinPointers.WF]
+  intro x hmemx
+  simp only [completeList, List.mem_map, Prod.exists] at hmemx
+  let P := fun x : BinItem T N => x.item.nextSymbol == some (Symbol.nonterminal y.rule.input)
+  let originBin := bins[y.startIdx]'(by grind)
+  let filteredOriginBin := filterWithIdx originBin P
+  simp only [Pointer.WF, ne_eq, tsub_le_iff_right]
+  -- z is the original item, which will be completed
+  rcases hmemx with ⟨z,zIdx,⟨hmemz,hx⟩⟩
+  have xP : x.pointer = Pointer.reduction ⟨y.startIdx, zIdx, j⟩ [] := by grind
+  simp only [xP]
+  refine ⟨by lia, by grind, ?_, by grind⟩
+  intro hbounds
+  exact filterWithIdx_le_length bins[y.startIdx]
+    (fun x => x.item.nextSymbol == some (Symbol.nonterminal y.rule.input)) zIdx (by grind)
+
+omit [LawfulBEq (EarleyItem T N)] in
+lemma soundPointers_of_completeList {G : ContextFreeGrammarList T N} (w : Array T) (j k : Nat)
+    (bins : EarleyBins T N (w.size + 1)) (hbins : EarleyBins.WF G bins) (y : EarleyItem T N)
+    (hk : k < bins.size) (hmemy : y ∈ (items bins[k])) (hj : j < bins[k].length) :
+    ∀ x ∈ completeList y bins (by grind) j, Pointer.isSound x.pointer k bins[k].length := by
+  simp only [Pointer.isSound]
+  intro x hmemx
+  simp only [completeList, List.mem_map, Prod.exists] at hmemx
+  let P := fun x : BinItem T N => x.item.nextSymbol == some (Symbol.nonterminal y.rule.input)
+  let originBin := bins[y.startIdx]'(by grind)
+  let filteredOriginBin := filterWithIdx originBin P
+  -- z is the original item, which will be completed
+  rcases hmemx with ⟨z,zIdx,⟨hmemz,hx⟩⟩
+  have xP : x.pointer = Pointer.reduction ⟨y.startIdx, zIdx, j⟩ [] := by grind
+  simp only [xP]
+  refine ⟨?_, by grind⟩
+  simp only [EarleyBins.WF, Order.lt_add_one_iff] at hbins
+  have : y.startIdx < k ∨ y.startIdx = k := by grind
+  rcases this with h | h
+  · grind
+  · simp only [h, lt_self_iff_false, true_and, false_or, gt_iff_lt]
+    exact filterWithIdx_le_length bins[k] P zIdx (by grind)
+
+theorem pointerWF_of_earleyList (G : ContextFreeGrammarList T N) (w : Array T) :
+    EarleyBins.PointerWF (earleyList G w).bins := by
+  sorry
+
+end Wellformed
 
 section Naive
 
@@ -84,15 +408,27 @@ def toGraphviz [ToString T] [ToString N] (t : Tree T N) : String :=
   graph ++ "\n}"
 
 omit [BEq T] [BEq N] in
-lemma wfPointerAux_of_redPointer {G : ContextFreeGrammarList T N} {w : Array T}
-    {endIdxA i j m n : Nat} {ps : List ReductionPointer}
-    {bins : EarleyBins T N (w.size + 1)} (hbins : EarleyBins.WF G bins)
+lemma wfPointerAux_of_predPointer {w : Array T} {i k j : Nat}
+    {bins : EarleyBins T N (w.size + 1)} (inv : EarleyBins.PointerWF bins)
+    (hk : k < w.size + 1) (hn : j < bins[k].length)
+    (h : bins[k][j].pointer = Pointer.predecessor i) :
+    k ≠ 0 ∧ k - 1 ≤ w.size ∧ ((h : k - 1 ≤ w.size) → i < bins[k-1].length) := by
+  specialize inv k hk
+  have ⟨pInv, _⟩ := inv
+  simp only [BinPointers.WF, Pointer.WF, ne_eq, tsub_le_iff_right] at pInv
+  specialize pInv bins[k][j] (by simp)
+  grind
+
+omit [BEq T] [BEq N] in
+lemma wfPointerAux_of_redPointer {w : Array T} {endIdxA i j m n : Nat} {ps : List ReductionPointer}
+    {bins : EarleyBins T N (w.size + 1)} (inv : EarleyBins.PointerWF bins)
     (hm : m < w.size + 1) (hn : n < bins[m].length)
     (h : bins[m][n].pointer = Pointer.reduction ⟨endIdxA, i, j⟩ ps) :
     endIdxA ≤ w.size ∧ j < bins[m].length ∧
     ∀ (h : endIdxA ≤ w.size), i < bins[endIdxA].length ∧
     (endIdxA < m ∨ (endIdxA = m ∧ i < n)) ∧ j < n := by
-  have ⟨_, _, pInv, sInv⟩:= hbins m (by lia)
+  specialize inv m hm
+  have ⟨pInv, sInv⟩ := inv
   simp only [BinPointers.WF, Pointer.WF, tsub_le_iff_right] at pInv
   specialize pInv bins[m][n] (by simp)
   simp only [h] at pInv
@@ -150,8 +486,9 @@ lemma foldl_le_of_le (xs : List Nat) (m k j : Nat) (hk : k < xs.length) (hjk : j
 Reconstruct the parse tree by searching the origin data from the EarleyBins.
 -/
 public def buildTree (G : ContextFreeGrammarList T N) (w : Array T) (hw : w ≠ #[])
-    (bins : EarleyBins T N (w.size + 1)) (inv : EarleyBins.WF G bins) (k : Nat)
-    (hk : k < w.size + 1) (j : Nat) (hj : j < bins[k].length) : Option (Tree T N) :=
+    (bins : EarleyBins T N (w.size + 1)) (hbins : EarleyBins.WF G bins)
+    (hwf : EarleyBins.PointerWF bins) (k : Nat) (hk : k < w.size + 1)
+    (j : Nat) (hj : j < bins[k].length) : Option (Tree T N) :=
   let binItem := bins[k][j]
   match hp : binItem.pointer with
   | .null =>
@@ -160,20 +497,19 @@ public def buildTree (G : ContextFreeGrammarList T N) (w : Array T) (hw : w ≠ 
   | .predecessor i => do
     -- Add sub tree starting from terminal
     have : k - 1 < w.size := by grind
-    have : i < bins[k - 1].length := by grind
-    let t ← buildTree G w hw bins inv (k-1) (by lia) i this
+    let t ← buildTree G w hw bins hbins hwf (k-1) (by lia) i (by grind)
     match t with
     | Tree.leaf d => none
     | Tree.node d ts =>
       some (Tree.node d (ts.append [Tree.leaf (Symbol.terminal w[k-1])]))
   | .reduction ⟨endIdxA,i,j⟩ ps => do
     -- We simply take the first possible parse tree.
-    have := wfPointerAux_of_redPointer inv _ _ hp
-    let t ← buildTree G w hw bins inv endIdxA (by lia) i (by lia)
+    have := wfPointerAux_of_redPointer hwf _ _ hp
+    let t ← buildTree G w hw bins hbins hwf endIdxA (by lia) i (by lia)
     match t with
     | Tree.leaf d => none
     | Tree.node d ts => do
-      let t ← buildTree G w hw bins inv k (by lia) j (by lia)
+      let t ← buildTree G w hw bins hbins hwf k (by lia) j (by lia)
       some (Tree.node d (ts.append [t]))
 -- Idea: if we go think of the two-dimensional bins as a continuous one-dimensional one,
 -- then each recursive call accesses a smaller index of the bin.
@@ -184,9 +520,9 @@ decreasing_by
         ((bins.toList.map List.length).take k).foldl Add.add 0 := by
       have := foldl_add_nth bins.toList 0 (k-1) (by grind)
       grind
-    lia
+    grind
   · rename Nat => pj
-    have : endIdxA < k ∨ (endIdxA = k ∧ i < j) := by grind [wfPointerAux_of_redPointer]
+    have : endIdxA < k ∨ (endIdxA = k ∧ i < j) := by grind
     rcases this with h | h
     · have : ((bins.toList.map List.length).take endIdxA).foldl Add.add 0 + bins[endIdxA].length ≤
              ((bins.toList.map List.length).take k).foldl Add.add 0 := by
@@ -195,7 +531,7 @@ decreasing_by
       lia
     · lia
   · rename Nat => pj
-    have : pj < j := by grind [wfPointerAux_of_redPointer]
+    have : pj < j := by grind
     simp [this]
 
 /--
@@ -208,14 +544,15 @@ public def parse [LawfulBEq (EarleyItem T N)] (G : ContextFreeGrammarList T N) (
   if hw : w = #[] then
     none
   else
-    let ⟨bins, inv⟩ := earleyList G w
+    let wfBins := earleyList G w
     -- Find the finished item, and follow its pointers.
     let P := fun x => isFinished G.initial w.size x.item
-    match h : filterWithIdx bins[w.size] P with
+    match h : filterWithIdx wfBins.bins[w.size] P with
     | [] => none
     | (_, i)::_ =>
-      have := filterWithIdx_le_length bins[w.size] P i (by grind)
-      buildTree G w hw bins inv w.size (by simp) i this
+      have inv := pointerWF_of_earleyList G w
+      have := filterWithIdx_le_length wfBins.bins[w.size] P i (by grind)
+      buildTree G w hw wfBins.bins wfBins.inv inv w.size (by simp) i this
 
 end Naive
 
@@ -224,10 +561,16 @@ section Cached
 open Earley.Model
 open Earley.Model.EarleyItem
 open Earley.CachedRecognizerPointers
+open Earley.Proofs.CachedRecognizerPointers
 open Earley.Utils
 
 variable {T N : Type} [BEq T] [BEq N] [LawfulBEq T] [LawfulBEq N] [LawfulBEq (EarleyItem T N)]
   [Hashable N] [Hashable (EarleyItem T N)]
+
+theorem pointerWF_of_earleyCached (G : ContextFreeGrammarList T N) (w : Array T) :
+    EarleyBins.PointerWF (rawList (earleyCached G w).bins) := by
+  have inv := pointerWF_of_earleyList G w
+  grind [earleyCachedBins_eq_earleyListBins]
 
 public def parseCached (G : ContextFreeGrammarList T N) (w : Array T) : Option (Tree T N) :=
   -- This could be inferred from the result of earleyList,
@@ -235,16 +578,17 @@ public def parseCached (G : ContextFreeGrammarList T N) (w : Array T) : Option (
   if hw : w = #[] then
     none
   else
-    let ⟨cachedBins, inv⟩ := earleyCached G w
-    let bins := rawList cachedBins
+    let wfBins := earleyCached G w
+    let bins := rawList wfBins.bins
     -- Find the finished item, and follow its pointers.
     let P := fun x => isFinished G.initial w.size x.item
     -- One _could_ use Array.findIdx here, but the implementation isn't actually more efficient.
     match h : filterWithIdx bins[w.size] P with
     | [] => none
     | (_, i)::_ =>
+      have inv := pointerWF_of_earleyCached G w
       have := filterWithIdx_le_length bins[w.size] P i (by grind)
-      buildTree G w (by grind) bins inv w.size (by simp) i this
+      buildTree G w (by grind) bins wfBins.inv inv w.size (by simp) i this
 
 end Cached
 end Parser
